Add ownership checks to memory loads and stores
In the extended compartmentalized memory model, load and store
operations (and their variants) take an additional parameter
representing the principal (component) that performs the operation. In
the simple model we are implementing, operations are allowed only if
the component owns the block, as given by the ownership information that
is already part of the memory.

The new ownership checks are added modularly to the relevant operations;
these are then propagated to related results. Many proofs need to be
modified, though typically the changes are straightforward. In general,
more case analysis is needed because conditions are more complex,
however the new sub-goals line up along predictable lines and the
main cases remain unchanged.

Perhaps the most interesting choice is that of compartments to add to
hypotheses and conclusions in modified lemmas: sometimes arbitrary,
sometimes limited to a distinguished component of interest, and other
times indifferent, though in practice bound by semantic constraints. In
some cases, ownership assumptions need to be added. These decisions will
need to be reviewed as the are used throughout the development, to make
their use as direct as possible.

common/Memory.v
@@ -200,6 +200,8 @@ Proof.
   apply perm_order'_dec.
 Defined.
 
+(* NOTE: RB: Keeping this limited to range checks instead of building in
+   ownership checks as well. *)
 Definition range_perm (m: mem) (b: block) (lo hi: Z) (k: perm_kind) (p: permission) : Prop :=
   forall ofs, lo <= ofs < hi -> perm m b ofs k p.
 
@@ -240,17 +242,32 @@ Proof.
   left; red; intros. omegaContradiction.
 Defined.
 
-(** [valid_access m chunk b ofs p] holds if a memory access
+(** [valid_access m chunk b ofs p cp] holds if a memory access
     of the given chunk is possible in [m] at address [b, ofs]
-    with current permissions [p].
+    with current permissions [p] and from compartment [cp].
     This means:
 - The range of bytes accessed all have current permission [p].
+- The block [b] belongs to the accessing compartment [cp].
 - The offset [ofs] is aligned.
 *)
 
+Definition own_block (m: mem) (b: block) (cp: compartment): Prop :=
+  PTree.get b (mem_compartments m) = Some cp.
+
+Remark own_block_dec:
+  forall m b cp, {own_block m b cp} + {~own_block m b cp}.
+Proof.
+  intros m b cp. unfold own_block.
+  destruct ((mem_compartments m) ! b) as [cp' |] eqn:Heq.
+  - destruct (Pos.eq_dec cp cp').
+    + left. subst. reflexivity.
+    + right. intro Hcontra. inv Hcontra. easy.
+  - right. easy.
+Defined.
+
 Definition valid_access (m: mem) (chunk: memory_chunk) (b: block) (ofs: Z) (p: permission) (cp: compartment): Prop :=
   range_perm m b ofs (ofs + size_chunk chunk) Cur p
-  /\ PTree.get b (mem_compartments m) = Some cp
+  /\ own_block m b cp
   /\ (align_chunk chunk | ofs).
 
 Theorem valid_access_implies:
@@ -493,9 +510,9 @@ Fixpoint getN (n: nat) (p: Z) (c: ZMap.t memval) {struct n}: list memval :=
   | S n' => ZMap.get p c :: getN n' (p + 1) c
   end.
 
-(** [load chunk m b ofs] perform a read in memory state [m], at address
-  [b] and offset [ofs].  It returns the value of the memory chunk
-  at that address.  [None] is returned if the accessed bytes
+(** [load chunk m b ofs cp] performs a read in memory state [m], at address
+  [b] and offset [ofs], from compartment [cp].  It returns the value of the
+  memory chunk at that address.  [None] is returned if the accessed bytes
   are not readable. *)
 
 Definition load (chunk: memory_chunk) (m: mem) (b: block) (ofs: Z) (cp: compartment): option val :=
@@ -503,7 +520,7 @@ Definition load (chunk: memory_chunk) (m: mem) (b: block) (ofs: Z) (cp: compartm
   then Some(decode_val chunk (getN (size_chunk_nat chunk) ofs (m.(mem_contents)#b)))
   else None.
 
-(** [loadv chunk m addr] is similar, but the address and offset are given
+(** [loadv chunk m addr cp] is similar, but the address and offset are given
   as a single value [addr], which must be a pointer value. *)
 
 Definition loadv (chunk: memory_chunk) (m: mem) (addr: val) (cp: compartment) : option val :=
@@ -512,12 +529,13 @@ Definition loadv (chunk: memory_chunk) (m: mem) (addr: val) (cp: compartment) : 
   | _ => None
   end.
 
-(** [loadbytes m b ofs n] reads [n] consecutive bytes starting at
+(** [loadbytes m b ofs n cp] reads [n] consecutive bytes starting at
   location [(b, ofs)].  Returns [None] if the accessed locations are
   not readable. *)
 
-Definition loadbytes (m: mem) (b: block) (ofs n: Z): option (list memval) :=
-  if range_perm_dec m b ofs (ofs + n) Cur Readable
+Definition loadbytes (m: mem) (b: block) (ofs n: Z) (cp: compartment): option (list memval) :=
+  if range_perm_dec m b ofs (ofs + n) Cur Readable &&
+     own_block_dec m b cp
   then Some (getN (Z.to_nat n) ofs (m.(mem_contents)#b))
   else None.
 
@@ -596,13 +614,14 @@ Proof.
   induction vl; simpl; intros. auto. rewrite IHvl. auto.
 Qed.
 
-(** [store chunk m b ofs v] perform a write in memory state [m].
-  Value [v] is stored at address [b] and offset [ofs].
+(** [store chunk m b ofs v cp] performs a write in memory state [m].
+  Value [v] is stored at address [b] and offset [ofs]
+  on behalf of component [cp].
   Return the updated memory store, or [None] if the accessed bytes
   are not writable. *)
 
-Program Definition store (chunk: memory_chunk) (m: mem) (b: block) (ofs: Z) (v: val): option mem :=
-  if valid_access_dec m chunk b ofs Writable then
+Program Definition store (chunk: memory_chunk) (m: mem) (b: block) (ofs: Z) (v: val) (cp : compartment): option mem :=
+  if valid_access_dec m chunk b ofs Writable cp then
     Some (mkmem (PMap.set b
                           (setN (encode_val chunk v) ofs (m.(mem_contents)#b))
                           m.(mem_contents))
@@ -623,21 +642,23 @@ Next Obligation.
   eapply nextblock_compartments.
 Qed.
 
-(** [storev chunk m addr v] is similar, but the address and offset are given
+(** [storev chunk m addr v cp] is similar, but the address and offset are given
   as a single value [addr], which must be a pointer value. *)
 
-Definition storev (chunk: memory_chunk) (m: mem) (addr v: val) : option mem :=
+Definition storev (chunk: memory_chunk) (m: mem) (addr v: val) (cp : compartment) : option mem :=
   match addr with
-  | Vptr b ofs => store chunk m b (Ptrofs.unsigned ofs) v
+  | Vptr b ofs => store chunk m b (Ptrofs.unsigned ofs) v cp
   | _ => None
   end.
 
-(** [storebytes m b ofs bytes] stores the given list of bytes [bytes]
-  starting at location [(b, ofs)].  Returns updated memory state
+(** [storebytes m b ofs bytes cp] has component [cp] store the given list of
+  bytes [bytes] starting at location [(b, ofs)].  Returns updated memory state
   or [None] if the accessed locations are not writable. *)
 
-Program Definition storebytes (m: mem) (b: block) (ofs: Z) (bytes: list memval) : option mem :=
-  if range_perm_dec m b ofs (ofs + Z.of_nat (length bytes)) Cur Writable then
+Program Definition storebytes (m: mem) (b: block) (ofs: Z) (bytes: list memval) (cp: compartment) : option mem :=
+  if range_perm_dec m b ofs (ofs + Z.of_nat (length bytes)) Cur Writable &&
+     own_block_dec m b cp
+  then
     Some (mkmem
              (PMap.set b (setN bytes ofs (m.(mem_contents)#b)) m.(mem_contents))
              m.(mem_access)
@@ -703,7 +724,7 @@ Proof.
   intros. unfold perm, empty; simpl. rewrite PMap.gi. simpl. tauto.
 Qed.
 
-Theorem valid_access_empty: forall chunk b ofs p, ~valid_access empty chunk b ofs p.
+Theorem valid_access_empty: forall chunk b ofs p cp, ~valid_access empty chunk b ofs p cp.
 Proof.
   intros. red; intros. elim (perm_empty b ofs Cur p). apply H.
   generalize (size_chunk_pos chunk); omega.
@@ -712,17 +733,17 @@ Qed.
 (** ** Properties related to [load] *)
 
 Theorem valid_access_load:
-  forall m chunk b ofs,
-  valid_access m chunk b ofs Readable ->
-  exists v, load chunk m b ofs = Some v.
+  forall m chunk b ofs cp,
+  valid_access m chunk b ofs Readable cp ->
+  exists v, load chunk m b ofs cp = Some v.
 Proof.
   intros. econstructor. unfold load. rewrite pred_dec_true; eauto.
 Qed.
 
 Theorem load_valid_access:
-  forall m chunk b ofs v,
-  load chunk m b ofs = Some v ->
-  valid_access m chunk b ofs Readable.
+  forall m chunk b ofs cp v,
+  load chunk m b ofs cp = Some v ->
+  valid_access m chunk b ofs Readable cp.
 Proof.
   intros until v. unfold load.
   destruct (valid_access_dec m chunk b ofs Readable); intros.
@@ -731,8 +752,8 @@ Proof.
 Qed.
 
 Lemma load_result:
-  forall chunk m b ofs v,
-  load chunk m b ofs = Some v ->
+  forall chunk m b ofs cp v,
+  load chunk m b ofs cp = Some v ->
   v = decode_val chunk (getN (size_chunk_nat chunk) ofs (m.(mem_contents)#b)).
 Proof.
   intros until v. unfold load.
@@ -744,8 +765,8 @@ Qed.
 Local Hint Resolve load_valid_access valid_access_load: mem.
 
 Theorem load_type:
-  forall m chunk b ofs v,
-  load chunk m b ofs = Some v ->
+  forall m chunk b ofs cp v,
+  load chunk m b ofs cp = Some v ->
   Val.has_type v (type_of_chunk chunk).
 Proof.
   intros. exploit load_result; eauto; intros. rewrite H0.
@@ -753,8 +774,8 @@ Proof.
 Qed.
 
 Theorem load_rettype:
-  forall m chunk b ofs v,
-  load chunk m b ofs = Some v ->
+  forall m chunk b ofs cp v,
+  load chunk m b ofs cp = Some v ->
   Val.has_rettype v (rettype_of_chunk chunk).
 Proof.
   intros. exploit load_result; eauto; intros. rewrite H0.
@@ -762,8 +783,8 @@ Proof.
 Qed.
 
 Theorem load_cast:
-  forall m chunk b ofs v,
-  load chunk m b ofs = Some v ->
+  forall m chunk b ofs cp v,
+  load chunk m b ofs cp = Some v ->
   match chunk with
   | Mint8signed => v = Val.sign_ext 8 v
   | Mint8unsigned => v = Val.zero_ext 8 v
@@ -778,8 +799,8 @@ Proof.
 Qed.
 
 Theorem load_int8_signed_unsigned:
-  forall m b ofs,
-  load Mint8signed m b ofs = option_map (Val.sign_ext 8) (load Mint8unsigned m b ofs).
+  forall m b ofs cp,
+  load Mint8signed m b ofs cp = option_map (Val.sign_ext 8) (load Mint8unsigned m b ofs cp).
 Proof.
   intros. unfold load.
   change (size_chunk_nat Mint8signed) with (size_chunk_nat Mint8unsigned).
@@ -792,8 +813,8 @@ Proof.
 Qed.
 
 Theorem load_int16_signed_unsigned:
-  forall m b ofs,
-  load Mint16signed m b ofs = option_map (Val.sign_ext 16) (load Mint16unsigned m b ofs).
+  forall m b ofs cp,
+  load Mint16signed m b ofs cp = option_map (Val.sign_ext 16) (load Mint16unsigned m b ofs cp).
 Proof.
   intros. unfold load.
   change (size_chunk_nat Mint16signed) with (size_chunk_nat Mint16unsigned).
@@ -808,45 +829,50 @@ Qed.
 (** ** Properties related to [loadbytes] *)
 
 Theorem range_perm_loadbytes:
-  forall m b ofs len,
+  forall m b ofs len cp,
   range_perm m b ofs (ofs + len) Cur Readable ->
-  exists bytes, loadbytes m b ofs len = Some bytes.
+  own_block m b cp ->
+  exists bytes, loadbytes m b ofs len cp = Some bytes.
 Proof.
-  intros. econstructor. unfold loadbytes. rewrite pred_dec_true; eauto.
+  intros. econstructor. unfold loadbytes. rewrite andb_lazy_alt.
+  setoid_rewrite pred_dec_true; eauto.
+  setoid_rewrite pred_dec_true; eauto.
 Qed.
 
 Theorem loadbytes_range_perm:
-  forall m b ofs len bytes,
-  loadbytes m b ofs len = Some bytes ->
+  forall m b ofs len cp bytes,
+  loadbytes m b ofs len cp = Some bytes ->
   range_perm m b ofs (ofs + len) Cur Readable.
 Proof.
   intros until bytes. unfold loadbytes.
-  destruct (range_perm_dec m b ofs (ofs + len) Cur Readable). auto. congruence.
+  destruct (range_perm_dec m b ofs (ofs + len) Cur Readable). auto. easy.
 Qed.
 
 Theorem loadbytes_load:
-  forall chunk m b ofs bytes,
-  loadbytes m b ofs (size_chunk chunk) = Some bytes ->
+  forall chunk m b ofs cp bytes,
+  loadbytes m b ofs (size_chunk chunk) cp = Some bytes ->
   (align_chunk chunk | ofs) ->
-  load chunk m b ofs = Some(decode_val chunk bytes).
+  load chunk m b ofs cp = Some(decode_val chunk bytes).
 Proof.
   unfold loadbytes, load; intros.
   destruct (range_perm_dec m b ofs (ofs + size_chunk chunk) Cur Readable);
-  try congruence.
-  inv H. rewrite pred_dec_true. auto.
-  split; auto.
+    destruct (own_block_dec m b cp);
+    inv H.
+  rewrite pred_dec_true. auto.
+  repeat split; auto.
 Qed.
 
 Theorem load_loadbytes:
-  forall chunk m b ofs v,
-  load chunk m b ofs = Some v ->
-  exists bytes, loadbytes m b ofs (size_chunk chunk) = Some bytes
+  forall chunk m b ofs cp v,
+  load chunk m b ofs cp = Some v ->
+  exists bytes, loadbytes m b ofs (size_chunk chunk) cp = Some bytes
              /\ v = decode_val chunk bytes.
 Proof.
-  intros. exploit load_valid_access; eauto. intros [A B].
+  intros. exploit load_valid_access; eauto. intros [A [B C]].
   exploit load_result; eauto. intros.
   exists (getN (size_chunk_nat chunk) ofs m.(mem_contents)#b); split.
-  unfold loadbytes. rewrite pred_dec_true; auto.
+  unfold loadbytes. rewrite andb_lazy_alt. setoid_rewrite pred_dec_true; auto.
+  setoid_rewrite pred_dec_true; auto.
   auto.
 Qed.
 
@@ -857,21 +883,34 @@ Proof.
 Qed.
 
 Theorem loadbytes_length:
-  forall m b ofs n bytes,
-  loadbytes m b ofs n = Some bytes ->
+  forall m b ofs n cp bytes,
+  loadbytes m b ofs n cp = Some bytes ->
   length bytes = Z.to_nat n.
 Proof.
   unfold loadbytes; intros.
-  destruct (range_perm_dec m b ofs (ofs + n) Cur Readable); try congruence.
-  inv H. apply getN_length.
+  destruct (range_perm_dec m b ofs (ofs + n) Cur Readable);
+    destruct (own_block_dec m b cp);
+    inv H;
+    try congruence.
+  apply getN_length.
 Qed.
 
+(* RB: NOTE: Had to add an [own_block] hypothesis here because that check is
+   part of the overall access check; Some nil and None may be somewhat similar,
+   but the difference seems significant. One could adjust the definition of
+   [loadbytes], but it is too early to measure the consequences of such a
+   change, which seems less principled, against the proofs that will need to
+   resort to this result. *)
 Theorem loadbytes_empty:
-  forall m b ofs n,
-  n <= 0 -> loadbytes m b ofs n = Some nil.
+  forall m b ofs n cp,
+  n <= 0 -> own_block m b cp -> loadbytes m b ofs n cp = Some nil.
 Proof.
-  intros. unfold loadbytes. rewrite pred_dec_true. rewrite Z_to_nat_neg; auto.
-  red; intros. omegaContradiction.
+  intros. unfold loadbytes. rewrite andb_lazy_alt.
+  setoid_rewrite pred_dec_true.
+  - destruct (own_block_dec m b cp).
+    + rewrite Z_to_nat_neg; auto.
+    + contradiction.
+  - red; intros. omegaContradiction.
 Qed.
 
 Lemma getN_concat:
@@ -886,49 +925,53 @@ Proof.
 Qed.
 
 Theorem loadbytes_concat:
-  forall m b ofs n1 n2 bytes1 bytes2,
-  loadbytes m b ofs n1 = Some bytes1 ->
-  loadbytes m b (ofs + n1) n2 = Some bytes2 ->
+  forall m b ofs n1 n2 cp bytes1 bytes2,
+  loadbytes m b ofs n1 cp = Some bytes1 ->
+  loadbytes m b (ofs + n1) n2 cp = Some bytes2 ->
   n1 >= 0 -> n2 >= 0 ->
-  loadbytes m b ofs (n1 + n2) = Some(bytes1 ++ bytes2).
+  loadbytes m b ofs (n1 + n2) cp = Some(bytes1 ++ bytes2).
 Proof.
   unfold loadbytes; intros.
-  destruct (range_perm_dec m b ofs (ofs + n1) Cur Readable); try congruence.
-  destruct (range_perm_dec m b (ofs + n1) (ofs + n1 + n2) Cur Readable); try congruence.
-  rewrite pred_dec_true. rewrite Z2Nat.inj_add by omega.
+  destruct (own_block_dec m b cp);
+    [| rewrite andb_comm in *; simpl in *; congruence].
+  destruct (range_perm_dec m b ofs (ofs + n1) Cur Readable); try (simpl in *; congruence).
+  destruct (range_perm_dec m b (ofs + n1) (ofs + n1 + n2) Cur Readable); try (simpl in *; congruence).
+  setoid_rewrite pred_dec_true. rewrite Z2Nat.inj_add by omega.
   rewrite getN_concat. rewrite Z2Nat.id by omega.
-  congruence.
+  simpl in *. congruence.
   red; intros.
   assert (ofs0 < ofs + n1 \/ ofs0 >= ofs + n1) by omega.
   destruct H4. apply r; omega. apply r0; omega.
 Qed.
 
 Theorem loadbytes_split:
-  forall m b ofs n1 n2 bytes,
-  loadbytes m b ofs (n1 + n2) = Some bytes ->
+  forall m b ofs n1 n2 cp bytes,
+  loadbytes m b ofs (n1 + n2) cp = Some bytes ->
   n1 >= 0 -> n2 >= 0 ->
   exists bytes1, exists bytes2,
-     loadbytes m b ofs n1 = Some bytes1
-  /\ loadbytes m b (ofs + n1) n2 = Some bytes2
+     loadbytes m b ofs n1 cp = Some bytes1
+  /\ loadbytes m b (ofs + n1) n2 cp = Some bytes2
   /\ bytes = bytes1 ++ bytes2.
 Proof.
   unfold loadbytes; intros.
+  destruct (own_block_dec m b cp);
+    [| rewrite andb_comm in *; simpl in *; congruence].
   destruct (range_perm_dec m b ofs (ofs + (n1 + n2)) Cur Readable);
-  try congruence.
+  try (simpl in *; congruence).
   rewrite Z2Nat.inj_add in H by omega. rewrite getN_concat in H.
   rewrite Z2Nat.id in H by omega.
-  repeat rewrite pred_dec_true.
+  repeat setoid_rewrite pred_dec_true.
   econstructor; econstructor.
-  split. reflexivity. split. reflexivity. congruence.
+  split. reflexivity. split. reflexivity. simpl in *. congruence.
   red; intros; apply r; omega.
   red; intros; apply r; omega.
 Qed.
 
 Theorem load_rep:
- forall ch m1 m2 b ofs v1 v2,
+ forall ch m1 m2 b ofs cp1 cp2 v1 v2,
   (forall z, 0 <= z < size_chunk ch -> ZMap.get (ofs + z) m1.(mem_contents)#b = ZMap.get (ofs + z) m2.(mem_contents)#b) ->
-  load ch m1 b ofs = Some v1 ->
-  load ch m2 b ofs = Some v2 ->
+  load ch m1 b ofs cp1 = Some v1 ->
+  load ch m2 b ofs cp2 = Some v2 ->
   v1 = v2.
 Proof.
   intros.
@@ -951,15 +994,15 @@ Proof.
 Qed.
 
 Theorem load_int64_split:
-  forall m b ofs v,
-  load Mint64 m b ofs = Some v -> Archi.ptr64 = false ->
+  forall m b ofs cp v,
+  load Mint64 m b ofs cp = Some v -> Archi.ptr64 = false ->
   exists v1 v2,
-     load Mint32 m b ofs = Some (if Archi.big_endian then v1 else v2)
-  /\ load Mint32 m b (ofs + 4) = Some (if Archi.big_endian then v2 else v1)
+     load Mint32 m b ofs cp = Some (if Archi.big_endian then v1 else v2)
+  /\ load Mint32 m b (ofs + 4) cp = Some (if Archi.big_endian then v2 else v1)
   /\ Val.lessdef v (Val.longofwords v1 v2).
 Proof.
   intros.
-  exploit load_valid_access; eauto. intros [A B]. simpl in *.
+  exploit load_valid_access; eauto. intros [A [B C]]. simpl in *.
   exploit load_loadbytes. eexact H. simpl. intros [bytes [LB EQ]].
   change 8 with (4 + 4) in LB.
   exploit loadbytes_split. eexact LB. omega. omega.
@@ -1002,11 +1045,11 @@ Proof.
 Qed.
 
 Theorem loadv_int64_split:
-  forall m a v,
-  loadv Mint64 m a = Some v -> Archi.ptr64 = false ->
+  forall m a cp v,
+  loadv Mint64 m a cp = Some v -> Archi.ptr64 = false ->
   exists v1 v2,
-     loadv Mint32 m a = Some (if Archi.big_endian then v1 else v2)
-  /\ loadv Mint32 m (Val.add a (Vint (Int.repr 4))) = Some (if Archi.big_endian then v2 else v1)
+     loadv Mint32 m a cp = Some (if Archi.big_endian then v1 else v2)
+  /\ loadv Mint32 m (Val.add a (Vint (Int.repr 4))) cp = Some (if Archi.big_endian then v2 else v1)
   /\ Val.lessdef v (Val.longofwords v1 v2).
 Proof.
   intros. destruct a; simpl in H; inv H.
@@ -1014,7 +1057,7 @@ Proof.
   unfold Val.add; rewrite H0.
   assert (NV: Ptrofs.unsigned (Ptrofs.add i (Ptrofs.of_int (Int.repr 4))) = Ptrofs.unsigned i + 4).
   { apply addressing_int64_split; auto.
-    exploit load_valid_access. eexact H2. intros [P Q]. auto. }
+    exploit load_valid_access. eexact H2. intros [P [Q R]]. auto. }
   exists v1, v2.
 Opaque Ptrofs.repr.
   split. auto.
@@ -1025,9 +1068,9 @@ Qed.
 (** ** Properties related to [store] *)
 
 Theorem valid_access_store:
-  forall m1 chunk b ofs v,
-  valid_access m1 chunk b ofs Writable ->
-  { m2: mem | store chunk m1 b ofs v = Some m2 }.
+  forall m1 chunk b ofs cp v,
+  valid_access m1 chunk b ofs Writable cp ->
+  { m2: mem | store chunk m1 b ofs v cp = Some m2 }.
 Proof.
   intros.
   unfold store.
@@ -1044,8 +1087,9 @@ Variable m1: mem.
 Variable b: block.
 Variable ofs: Z.
 Variable v: val.
+Variable cp : compartment.
 Variable m2: mem.
-Hypothesis STORE: store chunk m1 b ofs v = Some m2.
+Hypothesis STORE: store chunk m1 b ofs v cp = Some m2.
 
 Lemma store_access: mem_access m2 = mem_access m1.
 Proof.
@@ -1098,23 +1142,31 @@ Qed.
 Local Hint Resolve store_valid_block_1 store_valid_block_2: mem.
 
 Theorem store_valid_access_1:
-  forall chunk' b' ofs' p,
-  valid_access m1 chunk' b' ofs' p -> valid_access m2 chunk' b' ofs' p.
+  forall chunk' b' ofs' p cp,
+  valid_access m1 chunk' b' ofs' p cp -> valid_access m2 chunk' b' ofs' p cp.
 Proof.
-  intros. inv H. constructor; try red; auto with mem.
+  intros. inv H. destruct H1 as [H1 H2]. constructor; try red; auto with mem. split.
+  - unfold store in STORE.
+    destruct (valid_access_dec m1 chunk b ofs Writable cp); [| congruence].
+    inv STORE. auto.
+  - auto.
 Qed.
 
 Theorem store_valid_access_2:
-  forall chunk' b' ofs' p,
-  valid_access m2 chunk' b' ofs' p -> valid_access m1 chunk' b' ofs' p.
+  forall chunk' b' ofs' p cp',
+  valid_access m2 chunk' b' ofs' p cp' -> valid_access m1 chunk' b' ofs' p cp'.
 Proof.
-  intros. inv H. constructor; try red; auto with mem.
+  intros. inv H. destruct H1 as [H1 H2]. constructor; try red; auto with mem. split.
+  - unfold store in STORE.
+    destruct (valid_access_dec m1 chunk b ofs Writable cp); [| congruence].
+    inv STORE. auto.
+  - auto.
 Qed.
 
 Theorem store_valid_access_3:
-  valid_access m1 chunk b ofs Writable.
+  valid_access m1 chunk b ofs Writable cp.
 Proof.
-  unfold store in STORE. destruct (valid_access_dec m1 chunk b ofs Writable).
+  unfold store in STORE. destruct (valid_access_dec m1 chunk b ofs Writable cp).
   auto.
   congruence.
 Qed.
@@ -1135,7 +1187,7 @@ Theorem load_store_similar:
   forall chunk',
   size_chunk chunk' = size_chunk chunk ->
   align_chunk chunk' <= align_chunk chunk ->
-  exists v', load chunk' m2 b ofs = Some v' /\ decode_encode_val v chunk chunk' v'.
+  exists v', load chunk' m2 b ofs cp = Some v' /\ decode_encode_val v chunk chunk' v'.
 Proof.
   intros.
   exploit (valid_access_load m2 chunk').
@@ -1156,27 +1208,27 @@ Theorem load_store_similar_2:
   size_chunk chunk' = size_chunk chunk ->
   align_chunk chunk' <= align_chunk chunk ->
   type_of_chunk chunk' = type_of_chunk chunk ->
-  load chunk' m2 b ofs = Some (Val.load_result chunk' v).
+  load chunk' m2 b ofs cp = Some (Val.load_result chunk' v).
 Proof.
   intros. destruct (load_store_similar chunk') as [v' [A B]]; auto.
   rewrite A. decEq. eapply decode_encode_val_similar with (chunk1 := chunk); eauto.
 Qed.
 
 Theorem load_store_same:
-  load chunk m2 b ofs = Some (Val.load_result chunk v).
+  load chunk m2 b ofs cp = Some (Val.load_result chunk v).
 Proof.
   apply load_store_similar_2; auto. omega.
 Qed.
 
 Theorem load_store_other:
-  forall chunk' b' ofs',
+  forall chunk' b' ofs' cp',
   b' <> b
   \/ ofs' + size_chunk chunk' <= ofs
   \/ ofs + size_chunk chunk <= ofs' ->
-  load chunk' m2 b' ofs' = load chunk' m1 b' ofs'.
+  load chunk' m2 b' ofs' cp' = load chunk' m1 b' ofs' cp'.
 Proof.
   intros. unfold load.
-  destruct (valid_access_dec m1 chunk' b' ofs' Readable).
+  destruct (valid_access_dec m1 chunk' b' ofs' Readable cp').
   rewrite pred_dec_true.
   decEq. decEq. rewrite store_mem_contents; simpl.
   rewrite PMap.gsspec. destruct (peq b' b). subst b'.
@@ -1189,29 +1241,65 @@ Proof.
 Qed.
 
 Theorem loadbytes_store_same:
-  loadbytes m2 b ofs (size_chunk chunk) = Some(encode_val chunk v).
+  loadbytes m2 b ofs (size_chunk chunk) cp = Some(encode_val chunk v).
 Proof.
   intros.
-  assert (valid_access m2 chunk b ofs Readable) by eauto with mem.
-  unfold loadbytes. rewrite pred_dec_true. rewrite store_mem_contents; simpl.
+  assert (valid_access m2 chunk b ofs Readable cp) by eauto with mem.
+  destruct (own_block_dec m2 b cp);
+    [ | inversion H as [_ [Hcontra _]]; contradiction].
+  unfold loadbytes.
+  rewrite andb_lazy_alt. setoid_rewrite pred_dec_true. setoid_rewrite pred_dec_true.
+  rewrite store_mem_contents; simpl.
   rewrite PMap.gss.
   replace (Z.to_nat (size_chunk chunk)) with (length (encode_val chunk v)).
   rewrite getN_setN_same. auto.
   rewrite encode_val_length. auto.
+  auto.
   apply H.
 Qed.
 
-Theorem loadbytes_store_other:
+(* RB: NOTE: Split in _1 and _2 directions? *)
+Remark store_range_perm_inj :
   forall b' ofs' n,
+  range_perm m1 b' ofs' (ofs' + n) Cur Readable <->
+  range_perm m2 b' ofs' (ofs' + n) Cur Readable.
+Proof.
+  split; intros;
+    destruct (range_perm_dec m1 b' ofs' (ofs' + n) Cur Readable);
+    destruct (range_perm_dec m2 b' ofs' (ofs' + n) Cur Readable);
+    try contradiction; try assumption;
+    (unfold store in STORE;
+     destruct (valid_access_dec m1 chunk b ofs Writable cp);
+     inv STORE; now auto).
+Qed.
+
+(* RB: NOTE: Split in _1 and _2 directions? *)
+Remark store_own_block_inj :
+  forall b' cp',
+  own_block m1 b' cp' <-> own_block m2 b' cp'.
+Proof.
+  split; intros;
+    destruct (own_block_dec m1 b' cp');
+    destruct (own_block_dec m2 b' cp');
+    try contradiction; try assumption;
+    (unfold store in STORE;
+     destruct (valid_access_dec m1 chunk b ofs Writable cp);
+     inv STORE; now auto).
+Qed.
+
+Theorem loadbytes_store_other:
+  forall b' ofs' n cp',
   b' <> b
   \/ n <= 0
   \/ ofs' + n <= ofs
   \/ ofs + size_chunk chunk <= ofs' ->
-  loadbytes m2 b' ofs' n = loadbytes m1 b' ofs' n.
+  loadbytes m2 b' ofs' n cp' = loadbytes m1 b' ofs' n cp'.
 Proof.
   intros. unfold loadbytes.
   destruct (range_perm_dec m1 b' ofs' (ofs' + n) Cur Readable).
-  rewrite pred_dec_true.
+- rewrite andb_lazy_alt. setoid_rewrite pred_dec_true at 1.
++ destruct (own_block_dec m1 b' cp').
+* setoid_rewrite pred_dec_true. simpl.
   decEq. rewrite store_mem_contents; simpl.
   rewrite PMap.gsspec. destruct (peq b' b). subst b'.
   destruct H. congruence.
@@ -1221,9 +1309,13 @@ Proof.
   apply getN_setN_outside. rewrite encode_val_length. rewrite <- size_chunk_conv.
   rewrite Z2Nat.id. auto. omega.
   auto.
-  red; intros. eauto with mem.
-  rewrite pred_dec_false. auto.
-  red; intro; elim n0; red; intros; eauto with mem.
+  apply store_own_block_inj; auto.
+* setoid_rewrite pred_dec_false; auto.
+  intro Hcontra. apply store_own_block_inj in Hcontra. contradiction.
++ red; intros. eauto with mem.
+- setoid_rewrite pred_dec_false at 1.
++ auto.
++ red; intro; elim n0; red; intros; eauto with mem.
 Qed.
 
 Lemma setN_in:
@@ -1258,10 +1350,12 @@ Local Hint Resolve store_valid_block_1 store_valid_block_2: mem.
 Local Hint Resolve store_valid_access_1 store_valid_access_2
              store_valid_access_3: mem.
 
+(* RB: NOTE: [cp] and [cp'] must be equal, but the result does not rely on
+   this fact, and similarly for other related theorems. *)
 Lemma load_store_overlap:
-  forall chunk m1 b ofs v m2 chunk' ofs' v',
-  store chunk m1 b ofs v = Some m2 ->
-  load chunk' m2 b ofs' = Some v' ->
+  forall chunk m1 b ofs v cp m2 chunk' ofs' cp' v',
+  store chunk m1 b ofs v cp = Some m2 ->
+  load chunk' m2 b ofs' cp' = Some v' ->
   ofs' + size_chunk chunk' > ofs ->
   ofs + size_chunk chunk > ofs' ->
   exists mv1 mvl mv1' mvl',
@@ -1328,9 +1422,9 @@ Proof.
 Qed.
 
 Theorem load_pointer_store:
-  forall chunk m1 b ofs v m2 chunk' b' ofs' v_b v_o,
-  store chunk m1 b ofs v = Some m2 ->
-  load chunk' m2 b' ofs' = Some(Vptr v_b v_o) ->
+  forall chunk m1 b ofs v cp m2 chunk' b' ofs' cp' v_b v_o,
+  store chunk m1 b ofs v cp = Some m2 ->
+  load chunk' m2 b' ofs' cp' = Some(Vptr v_b v_o) ->
   (v = Vptr v_b v_o /\ compat_pointer_chunks chunk chunk' /\ b' = b /\ ofs' = ofs)
   \/ (b' <> b \/ ofs' + size_chunk chunk' <= ofs \/ ofs + size_chunk chunk <= ofs').
 Proof.
@@ -1361,9 +1455,9 @@ Proof.
 Qed.
 
 Theorem load_store_pointer_overlap:
-  forall chunk m1 b ofs v_b v_o m2 chunk' ofs' v,
-  store chunk m1 b ofs (Vptr v_b v_o) = Some m2 ->
-  load chunk' m2 b ofs' = Some v ->
+  forall chunk m1 b ofs v_b v_o cp m2 chunk' ofs' cp' v,
+  store chunk m1 b ofs (Vptr v_b v_o) cp = Some m2 ->
+  load chunk' m2 b ofs' cp' = Some v ->
   ofs' <> ofs ->
   ofs' + size_chunk chunk' > ofs ->
   ofs + size_chunk chunk > ofs' ->
@@ -1385,9 +1479,9 @@ Proof.
 Qed.
 
 Theorem load_store_pointer_mismatch:
-  forall chunk m1 b ofs v_b v_o m2 chunk' v,
-  store chunk m1 b ofs (Vptr v_b v_o) = Some m2 ->
-  load chunk' m2 b ofs = Some v ->
+  forall chunk m1 b ofs v_b v_o cp m2 cp' chunk' v,
+  store chunk m1 b ofs (Vptr v_b v_o) cp = Some m2 ->
+  load chunk' m2 b ofs cp' = Some v ->
   ~compat_pointer_chunks chunk chunk' ->
   v = Vundef.
 Proof.
@@ -1403,10 +1497,10 @@ Proof.
 Qed.
 
 Lemma store_similar_chunks:
-  forall chunk1 chunk2 v1 v2 m b ofs,
+  forall chunk1 chunk2 v1 v2 m b ofs cp,
   encode_val chunk1 v1 = encode_val chunk2 v2 ->
   align_chunk chunk1 = align_chunk chunk2 ->
-  store chunk1 m b ofs v1 = store chunk2 m b ofs v2.
+  store chunk1 m b ofs v1 cp = store chunk2 m b ofs v2 cp.
 Proof.
   intros. unfold store.
   assert (size_chunk chunk1 = size_chunk chunk2).
@@ -1423,37 +1517,37 @@ Proof.
 Qed.
 
 Theorem store_signed_unsigned_8:
-  forall m b ofs v,
-  store Mint8signed m b ofs v = store Mint8unsigned m b ofs v.
+  forall m b ofs v cp,
+  store Mint8signed m b ofs v cp = store Mint8unsigned m b ofs v cp.
 Proof. intros. apply store_similar_chunks. apply encode_val_int8_signed_unsigned. auto. Qed.
 
 Theorem store_signed_unsigned_16:
-  forall m b ofs v,
-  store Mint16signed m b ofs v = store Mint16unsigned m b ofs v.
+  forall m b ofs v cp,
+  store Mint16signed m b ofs v cp = store Mint16unsigned m b ofs v cp.
 Proof. intros. apply store_similar_chunks. apply encode_val_int16_signed_unsigned. auto. Qed.
 
 Theorem store_int8_zero_ext:
-  forall m b ofs n,
-  store Mint8unsigned m b ofs (Vint (Int.zero_ext 8 n)) =
-  store Mint8unsigned m b ofs (Vint n).
+  forall m b ofs n cp,
+  store Mint8unsigned m b ofs (Vint (Int.zero_ext 8 n)) cp =
+  store Mint8unsigned m b ofs (Vint n) cp.
 Proof. intros. apply store_similar_chunks. apply encode_val_int8_zero_ext. auto. Qed.
 
 Theorem store_int8_sign_ext:
-  forall m b ofs n,
-  store Mint8signed m b ofs (Vint (Int.sign_ext 8 n)) =
-  store Mint8signed m b ofs (Vint n).
+  forall m b ofs n cp,
+  store Mint8signed m b ofs (Vint (Int.sign_ext 8 n)) cp =
+  store Mint8signed m b ofs (Vint n) cp.
 Proof. intros. apply store_similar_chunks. apply encode_val_int8_sign_ext. auto. Qed.
 
 Theorem store_int16_zero_ext:
-  forall m b ofs n,
-  store Mint16unsigned m b ofs (Vint (Int.zero_ext 16 n)) =
-  store Mint16unsigned m b ofs (Vint n).
+  forall m b ofs n cp,
+  store Mint16unsigned m b ofs (Vint (Int.zero_ext 16 n)) cp =
+  store Mint16unsigned m b ofs (Vint n) cp.
 Proof. intros. apply store_similar_chunks. apply encode_val_int16_zero_ext. auto. Qed.
 
 Theorem store_int16_sign_ext:
-  forall m b ofs n,
-  store Mint16signed m b ofs (Vint (Int.sign_ext 16 n)) =
-  store Mint16signed m b ofs (Vint n).
+  forall m b ofs n cp,
+  store Mint16signed m b ofs (Vint (Int.sign_ext 16 n)) cp =
+  store Mint16signed m b ofs (Vint n) cp.
 Proof. intros. apply store_similar_chunks. apply encode_val_int16_sign_ext. auto. Qed.
 
 (*
@@ -1478,24 +1572,29 @@ Qed.
 
 (** ** Properties related to [storebytes]. *)
 
+(* RB: NOTE: Like [loadbytes], [storebytes] builds in the ownership check and
+   some results are best complemented by ownership hypotheses, at least at this
+   stage. *)
 Theorem range_perm_storebytes:
-  forall m1 b ofs bytes,
+  forall m1 b ofs bytes cp,
   range_perm m1 b ofs (ofs + Z.of_nat (length bytes)) Cur Writable ->
-  { m2 : mem | storebytes m1 b ofs bytes = Some m2 }.
+  own_block m1 b cp ->
+  { m2 : mem | storebytes m1 b ofs bytes cp = Some m2 }.
 Proof.
   intros. unfold storebytes.
   destruct (range_perm_dec m1 b ofs (ofs + Z.of_nat (length bytes)) Cur Writable).
-  econstructor; reflexivity.
+  econstructor. setoid_rewrite pred_dec_true. reflexivity. assumption.
   contradiction.
 Defined.
 
 Theorem storebytes_store:
-  forall m1 b ofs chunk v m2,
-  storebytes m1 b ofs (encode_val chunk v) = Some m2 ->
+  forall m1 b ofs chunk v m2 cp,
+  storebytes m1 b ofs (encode_val chunk v) cp = Some m2 ->
   (align_chunk chunk | ofs) ->
-  store chunk m1 b ofs v = Some m2.
+  store chunk m1 b ofs v cp = Some m2.
 Proof.
   unfold storebytes, store. intros.
+  destruct (own_block_dec m1 b cp); [| rewrite andb_false_r in H; now inversion H].
   destruct (range_perm_dec m1 b ofs (ofs + Z.of_nat (length (encode_val chunk v))) Cur Writable); inv H.
   destruct (valid_access_dec m1 chunk b ofs Writable).
   f_equal. apply mkmem_ext; auto.
@@ -1504,13 +1603,16 @@ Proof.
 Qed.
 
 Theorem store_storebytes:
-  forall m1 b ofs chunk v m2,
-  store chunk m1 b ofs v = Some m2 ->
-  storebytes m1 b ofs (encode_val chunk v) = Some m2.
+  forall m1 b ofs chunk v cp m2,
+  store chunk m1 b ofs v cp = Some m2 ->
+  storebytes m1 b ofs (encode_val chunk v) cp = Some m2.
 Proof.
   unfold storebytes, store. intros.
   destruct (valid_access_dec m1 chunk b ofs Writable); inv H.
+  inversion v0 as [_ [Hown _]].
+  destruct (own_block_dec m1 b cp); [| contradiction].
   destruct (range_perm_dec m1 b ofs (ofs + Z.of_nat (length (encode_val chunk v))) Cur Writable).
+  simpl.
   f_equal. apply mkmem_ext; auto.
   destruct v0.  elim n.
   rewrite encode_val_length. rewrite <- size_chunk_conv. auto.
@@ -1521,13 +1623,60 @@ Variable m1: mem.
 Variable b: block.
 Variable ofs: Z.
 Variable bytes: list memval.
+Variable cp: compartment.
 Variable m2: mem.
-Hypothesis STORE: storebytes m1 b ofs bytes = Some m2.
+Hypothesis STORE: storebytes m1 b ofs bytes cp = Some m2.
+
+Lemma storebytes_own_block_1 : own_block m1 b cp.
+Proof.
+  unfold storebytes in STORE.
+  destruct (range_perm_dec m1 b ofs (ofs + Z.of_nat (Datatypes.length bytes)) Cur Writable);
+    [| now inversion STORE].
+  destruct (own_block_dec m1 b cp);
+    [| now inversion STORE].
+  assumption.
+Qed.
+
+Lemma storebytes_own_block_2 : own_block m2 b cp.
+Proof.
+  unfold storebytes in STORE.
+  destruct (range_perm_dec m1 b ofs (ofs + Z.of_nat (Datatypes.length bytes)) Cur Writable);
+    [| now inversion STORE].
+  destruct (own_block_dec m1 b cp);
+    inv STORE.
+  assumption.
+Qed.
+
+(* RB: NOTE: Names and split adapted from storebytes_valid_block_1 and _2 below,
+   similar auxiliary results could follow the same pattern (with preservation
+   suffix, see lemmas above). *)
+Lemma storebytes_own_block_inj_1 :
+  forall b' cp', own_block m1 b' cp' -> own_block m2 b' cp'.
+Proof.
+  unfold own_block, storebytes in *;
+    intros b' cp' H;
+    destruct (range_perm_dec m1 b ofs (ofs + Z.of_nat (Datatypes.length bytes)) Cur Writable);
+    destruct (own_block_dec m1 b cp);
+    inv STORE;
+    assumption.
+Qed.
+
+Lemma storebytes_own_block_inj_2 :
+  forall b' cp', own_block m2 b' cp' -> own_block m1 b' cp'.
+Proof.
+  unfold own_block, storebytes in *;
+    intros b' cp' H;
+    destruct (range_perm_dec m1 b ofs (ofs + Z.of_nat (Datatypes.length bytes)) Cur Writable);
+    destruct (own_block_dec m1 b cp);
+    inv STORE;
+    assumption.
+Qed.
 
 Lemma storebytes_access: mem_access m2 = mem_access m1.
 Proof.
   unfold storebytes in STORE.
   destruct (range_perm_dec m1 b ofs (ofs + Z.of_nat (length bytes)) Cur Writable);
+  destruct (own_block_dec m1 b cp);
   inv STORE.
   auto.
 Qed.
@@ -1537,6 +1686,7 @@ Lemma storebytes_mem_contents:
 Proof.
   unfold storebytes in STORE.
   destruct (range_perm_dec m1 b ofs (ofs + Z.of_nat (length bytes)) Cur Writable);
+  destruct (own_block_dec m1 b cp);
   inv STORE.
   auto.
 Qed.
@@ -1556,17 +1706,21 @@ Qed.
 Local Hint Resolve perm_storebytes_1 perm_storebytes_2: mem.
 
 Theorem storebytes_valid_access_1:
-  forall chunk' b' ofs' p,
-  valid_access m1 chunk' b' ofs' p -> valid_access m2 chunk' b' ofs' p.
+  forall chunk' b' ofs' p cp',
+  valid_access m1 chunk' b' ofs' p cp' -> valid_access m2 chunk' b' ofs' p cp'.
 Proof.
-  intros. inv H. constructor; try red; auto with mem.
+  intros. inv H. destruct H1 as [H1 H2]. constructor; try red; auto with mem.
+  split; auto.
+  apply storebytes_own_block_inj_1; eassumption.
 Qed.
 
 Theorem storebytes_valid_access_2:
-  forall chunk' b' ofs' p,
-  valid_access m2 chunk' b' ofs' p -> valid_access m1 chunk' b' ofs' p.
+  forall chunk' b' ofs' p cp',
+  valid_access m2 chunk' b' ofs' p cp' -> valid_access m1 chunk' b' ofs' p cp'.
 Proof.
-  intros. inv H. constructor; try red; auto with mem.
+  intros. inv H. destruct H1 as [H1 H2]. constructor; try red; auto with mem.
+  split; auto.
+  apply storebytes_own_block_inj_2; eassumption.
 Qed.
 
 Local Hint Resolve storebytes_valid_access_1 storebytes_valid_access_2: mem.
@@ -1577,6 +1731,7 @@ Proof.
   intros.
   unfold storebytes in STORE.
   destruct (range_perm_dec m1 b ofs (ofs + Z.of_nat (length bytes)) Cur Writable);
+  destruct (own_block_dec m1 b cp);
   inv STORE.
   auto.
 Qed.
@@ -1606,64 +1761,79 @@ Proof.
 Qed.
 
 Theorem loadbytes_storebytes_same:
-  loadbytes m2 b ofs (Z.of_nat (length bytes)) = Some bytes.
+  loadbytes m2 b ofs (Z.of_nat (length bytes)) cp = Some bytes.
 Proof.
   intros. assert (STORE2:=STORE). unfold storebytes in STORE2. unfold loadbytes.
   destruct (range_perm_dec m1 b ofs (ofs + Z.of_nat (length bytes)) Cur Writable);
+  destruct (own_block_dec m1 b cp);
   try discriminate.
-  rewrite pred_dec_true.
+  setoid_rewrite pred_dec_true. simpl.
   decEq. inv STORE2; simpl. rewrite PMap.gss. rewrite Nat2Z.id.
   apply getN_setN_same.
   red; eauto with mem.
+  apply storebytes_own_block_inj_1; eassumption.
 Qed.
 
 Theorem loadbytes_storebytes_disjoint:
-  forall b' ofs' len,
+  forall b' ofs' len cp',
   len >= 0 ->
   b' <> b \/ Intv.disjoint (ofs', ofs' + len) (ofs, ofs + Z.of_nat (length bytes)) ->
-  loadbytes m2 b' ofs' len = loadbytes m1 b' ofs' len.
+  loadbytes m2 b' ofs' len cp' = loadbytes m1 b' ofs' len cp'.
 Proof.
   intros. unfold loadbytes.
-  destruct (range_perm_dec m1 b' ofs' (ofs' + len) Cur Readable).
-  rewrite pred_dec_true.
-  rewrite storebytes_mem_contents. decEq.
+  destruct (range_perm_dec m1 b' ofs' (ofs' + len) Cur Readable);
+  destruct (own_block_dec m1 b' cp').
+- setoid_rewrite pred_dec_true; simpl.
++ rewrite storebytes_mem_contents. decEq.
   rewrite PMap.gsspec. destruct (peq b' b). subst b'.
   apply getN_setN_disjoint. rewrite Z2Nat.id by omega. intuition congruence.
   auto.
-  red; auto with mem.
-  apply pred_dec_false.
++ red; auto with mem.
++ apply storebytes_own_block_inj_1; assumption.
+- setoid_rewrite pred_dec_false at 2.
++ do 2 rewrite andb_false_r. reflexivity.
++ intro Hcontra. apply storebytes_own_block_inj_2 in Hcontra. contradiction.
+- setoid_rewrite pred_dec_false at 1; simpl. reflexivity.
+  red; intros; elim n. red; auto with mem.
+- setoid_rewrite pred_dec_false at 1; simpl. reflexivity.
   red; intros; elim n. red; auto with mem.
 Qed.
 
 Theorem loadbytes_storebytes_other:
-  forall b' ofs' len,
+  forall b' ofs' len cp',
   len >= 0 ->
   b' <> b
   \/ ofs' + len <= ofs
   \/ ofs + Z.of_nat (length bytes) <= ofs' ->
-  loadbytes m2 b' ofs' len = loadbytes m1 b' ofs' len.
+  loadbytes m2 b' ofs' len cp' = loadbytes m1 b' ofs' len cp'.
 Proof.
   intros. apply loadbytes_storebytes_disjoint; auto.
   destruct H0; auto. right. apply Intv.disjoint_range; auto.
 Qed.
 
 Theorem load_storebytes_other:
-  forall chunk b' ofs',
+  forall chunk b' ofs' cp',
   b' <> b
   \/ ofs' + size_chunk chunk <= ofs
   \/ ofs + Z.of_nat (length bytes) <= ofs' ->
-  load chunk m2 b' ofs' = load chunk m1 b' ofs'.
+  load chunk m2 b' ofs' cp' = load chunk m1 b' ofs' cp'.
 Proof.
   intros. unfold load.
-  destruct (valid_access_dec m1 chunk b' ofs' Readable).
+  destruct (valid_access_dec m1 chunk b' ofs' Readable cp').
   rewrite pred_dec_true.
   rewrite storebytes_mem_contents. decEq.
   rewrite PMap.gsspec. destruct (peq b' b). subst b'.
   rewrite getN_setN_outside. auto. rewrite <- size_chunk_conv. intuition congruence.
   auto.
   destruct v; split; auto. red; auto with mem.
+  destruct H1 as [H1 H2]. split.
+  apply storebytes_own_block_inj_1; assumption.
+  assumption.
   apply pred_dec_false.
   red; intros; elim n. destruct H0. split; auto. red; auto with mem.
+  destruct H1 as [H1 H2]. split.
+  apply storebytes_own_block_inj_2; assumption.
+  assumption.
 Qed.
 
 End STOREBYTES.
@@ -1677,16 +1847,24 @@ Proof.
   simpl length. rewrite Nat2Z.inj_succ. simpl. rewrite IHbytes1. decEq. omega.
 Qed.
 
+(* RB: NOTE: Different compartment variables could be used in each premise (and
+   the conclusion), as those would effectively be equal. *)
 Theorem storebytes_concat:
-  forall m b ofs bytes1 m1 bytes2 m2,
-  storebytes m b ofs bytes1 = Some m1 ->
-  storebytes m1 b (ofs + Z.of_nat(length bytes1)) bytes2 = Some m2 ->
-  storebytes m b ofs (bytes1 ++ bytes2) = Some m2.
+  forall m b ofs bytes1 cp m1 bytes2 m2,
+  storebytes m b ofs bytes1 cp = Some m1 ->
+  storebytes m1 b (ofs + Z.of_nat(length bytes1)) bytes2 cp = Some m2 ->
+  storebytes m b ofs (bytes1 ++ bytes2) cp = Some m2.
 Proof.
   intros. generalize H; intro ST1. generalize H0; intro ST2.
   unfold storebytes; unfold storebytes in ST1; unfold storebytes in ST2.
-  destruct (range_perm_dec m b ofs (ofs + Z.of_nat(length bytes1)) Cur Writable); try congruence.
-  destruct (range_perm_dec m1 b (ofs + Z.of_nat(length bytes1)) (ofs + Z.of_nat(length bytes1) + Z.of_nat(length bytes2)) Cur Writable); try congruence.
+  destruct (range_perm_dec m b ofs (ofs + Z.of_nat(length bytes1)) Cur Writable);
+  destruct (own_block_dec m b cp);
+  simpl in *;
+  try congruence.
+  destruct (range_perm_dec m1 b (ofs + Z.of_nat(length bytes1)) (ofs + Z.of_nat(length bytes1) + Z.of_nat(length bytes2)) Cur Writable);
+  destruct (own_block_dec m1 b cp);
+  simpl in *;
+  try congruence.
   destruct (range_perm_dec m b ofs (ofs + Z.of_nat (length (bytes1 ++ bytes2))) Cur Writable).
   inv ST1; inv ST2; simpl. decEq. apply mkmem_ext; auto.
   rewrite PMap.gss.  rewrite setN_concat. symmetry. apply PMap.set2.
@@ -1698,20 +1876,22 @@ Proof.
 Qed.
 
 Theorem storebytes_split:
-  forall m b ofs bytes1 bytes2 m2,
-  storebytes m b ofs (bytes1 ++ bytes2) = Some m2 ->
+  forall m b ofs bytes1 bytes2 cp m2,
+  storebytes m b ofs (bytes1 ++ bytes2) cp = Some m2 ->
   exists m1,
-     storebytes m b ofs bytes1 = Some m1
-  /\ storebytes m1 b (ofs + Z.of_nat(length bytes1)) bytes2 = Some m2.
+     storebytes m b ofs bytes1 cp = Some m1
+  /\ storebytes m1 b (ofs + Z.of_nat(length bytes1)) bytes2 cp = Some m2.
 Proof.
   intros.
-  destruct (range_perm_storebytes m b ofs bytes1) as [m1 ST1].
+  destruct (range_perm_storebytes m b ofs bytes1 cp) as [m1 ST1].
   red; intros. exploit storebytes_range_perm; eauto. rewrite app_length.
   rewrite Nat2Z.inj_add. omega.
-  destruct (range_perm_storebytes m1 b (ofs + Z.of_nat (length bytes1)) bytes2) as [m2' ST2].
+  eapply storebytes_own_block_1; eassumption.
+  destruct (range_perm_storebytes m1 b (ofs + Z.of_nat (length bytes1)) bytes2 cp) as [m2' ST2].
   red; intros. eapply perm_storebytes_1; eauto. exploit storebytes_range_perm.
   eexact H. instantiate (1 := ofs0). rewrite app_length. rewrite Nat2Z.inj_add. omega.
   auto.
+  eapply storebytes_own_block_2; eassumption.
   assert (Some m2 = Some m2').
   rewrite <- H. eapply storebytes_concat; eauto.
   inv H0.
@@ -1719,14 +1899,14 @@ Proof.
 Qed.
 
 Theorem store_int64_split:
-  forall m b ofs v m',
-  store Mint64 m b ofs v = Some m' -> Archi.ptr64 = false ->
+  forall m b ofs v cp m',
+  store Mint64 m b ofs v cp = Some m' -> Archi.ptr64 = false ->
   exists m1,
-     store Mint32 m b ofs (if Archi.big_endian then Val.hiword v else Val.loword v) = Some m1
-  /\ store Mint32 m1 b (ofs + 4) (if Archi.big_endian then Val.loword v else Val.hiword v) = Some m'.
+     store Mint32 m b ofs (if Archi.big_endian then Val.hiword v else Val.loword v) cp = Some m1
+  /\ store Mint32 m1 b (ofs + 4) (if Archi.big_endian then Val.loword v else Val.hiword v) cp = Some m'.
 Proof.
   intros.
-  exploit store_valid_access_3; eauto. intros [A B]. simpl in *.
+  exploit store_valid_access_3; eauto. intros [A [B C]]. simpl in *.
   exploit store_storebytes. eexact H. intros SB.
   rewrite encode_val_int64 in SB by auto.
   exploit storebytes_split. eexact SB. intros [m1 [SB1 SB2]].
@@ -1739,11 +1919,11 @@ Proof.
 Qed.
 
 Theorem storev_int64_split:
-  forall m a v m',
-  storev Mint64 m a v = Some m' -> Archi.ptr64 = false ->
+  forall m a v cp m',
+  storev Mint64 m a v cp = Some m' -> Archi.ptr64 = false ->
   exists m1,
-     storev Mint32 m a (if Archi.big_endian then Val.hiword v else Val.loword v) = Some m1
-  /\ storev Mint32 m1 (Val.add a (Vint (Int.repr 4))) (if Archi.big_endian then Val.loword v else Val.hiword v) = Some m'.
+     storev Mint32 m a (if Archi.big_endian then Val.hiword v else Val.loword v) cp = Some m1
+  /\ storev Mint32 m1 (Val.add a (Vint (Int.repr 4))) (if Archi.big_endian then Val.loword v else Val.hiword v) cp = Some m'.
 Proof.
   intros. destruct a; simpl in H; inv H. rewrite H2.
   exploit store_int64_split; eauto. intros [m1 [A B]].
@@ -1751,7 +1931,7 @@ Proof.
   exact A.
   unfold storev, Val.add. rewrite H0.
   rewrite addressing_int64_split; auto.
-  exploit store_valid_access_3. eexact H2. intros [P Q]. exact Q.
+  exploit store_valid_access_3. eexact H2. intros [P [R Q]]. exact Q.
 Qed.
 
 (** ** Properties related to [alloc]. *)
@@ -1796,6 +1976,32 @@ Proof.
   unfold valid_block. rewrite alloc_result. rewrite nextblock_alloc. apply Plt_succ.
 Qed.
 
+(* RB: NOTE: Maybe add these new lemmas to hint databases. *)
+Lemma alloc_mem_compartments_nextblock :
+  (mem_compartments m1) ! (nextblock m1) = None.
+Proof.
+  unfold alloc in ALLOC. destruct m1. inv ALLOC. simpl in *.
+  apply nextblock_compartments0. apply Plt_strict.
+Qed.
+
+Theorem unowned_fresh_block:
+  ~own_block m1 b c.
+Proof.
+  unfold own_block. intro Hcontra.
+  unfold alloc in ALLOC. destruct m1. inv ALLOC. simpl in *.
+  rewrite (proj1 (nextblock_compartments0 b)) in Hcontra.
+  - inversion Hcontra.
+  - apply Plt_strict.
+Qed.
+
+Theorem owned_new_block:
+  own_block m2 b c.
+Proof.
+  unfold own_block.
+  unfold alloc in ALLOC. destruct m1. inv ALLOC. simpl in *.
+  apply PTree.gss.
+Qed.
+
 Local Hint Resolve valid_block_alloc fresh_block_alloc valid_new_block: mem.
 
 Theorem valid_block_alloc_inv:
@@ -1804,6 +2010,13 @@ Proof.
   unfold valid_block; intros.
   rewrite nextblock_alloc in H. rewrite alloc_result.
   exploit Plt_succ_inv; eauto. tauto.
+Qed.
+
+Theorem valid_block_alloc_inv':
+  forall b', valid_block m1 b' -> b' <> b.
+Proof.
+  intros b' Hvalid Heq; subst b'.
+  apply fresh_block_alloc. assumption.
 Qed.
 
 Theorem perm_alloc_1:
@@ -1848,34 +2061,73 @@ Qed.
 
 Local Hint Resolve perm_alloc_1 perm_alloc_2 perm_alloc_3 perm_alloc_4: mem.
 
-Theorem valid_access_alloc_other:
-  forall chunk b' ofs p,
-  valid_access m1 chunk b' ofs p ->
-  valid_access m2 chunk b' ofs p.
+Lemma alloc_own_block_inj :
+  forall b' c', own_block m1 b' c' -> b <> b'.
 Proof.
-  intros. inv H. constructor; auto with mem.
+  intros b' c' Hown Heq; subst b'.
+  unfold own_block in Hown.
+  unfold alloc in ALLOC. destruct m1. inv ALLOC. simpl in *.
+  rewrite (proj1 (nextblock_compartments0 b)) in Hown.
+  - inversion Hown.
+  - apply Plt_strict.
+Qed.
+
+Lemma alloc_own_block_other_inj_1 :
+  forall b' c', own_block m1 b' c' -> own_block m2 b' c'.
+Proof.
+  unfold own_block. intros b' c' Hown.
+  pose proof alloc_mem_compartments_nextblock as Hnone. (* Pose to avoid silly error below. *)
+  inversion ALLOC; subst.
+  simpl in *.
+  destruct (own_block_dec m1 (nextblock m1) c).
+  - unfold own_block in o.
+    rewrite Hnone in o. (* Could not rewrite without having added this to the context. *)
+    inv o.
+  - rewrite <- Hown. apply PTree.gso. congruence.
+Qed.
+
+Lemma alloc_own_block_other_inj_2 :
+  forall b' c', b' <> b -> own_block m2 b' c' -> own_block m1 b' c'.
+Proof.
+  unfold own_block. intros b' c' Hneq Hown.
+  inversion ALLOC; subst. simpl in *.
+  rewrite <- Hown. symmetry. apply PTree.gso. assumption.
+Qed.
+
+Theorem valid_access_alloc_other:
+  forall chunk b' ofs p c',
+  valid_access m1 chunk b' ofs p c' ->
+  valid_access m2 chunk b' ofs p c'.
+Proof.
+  intros. inv H. destruct H1 as [H1 H2]. constructor; auto with mem.
   red; auto with mem.
+  split.
+  apply alloc_own_block_other_inj_1; assumption.
+  auto.
 Qed.
 
 Theorem valid_access_alloc_same:
   forall chunk ofs,
   lo <= ofs -> ofs + size_chunk chunk <= hi -> (align_chunk chunk | ofs) ->
-  valid_access m2 chunk b ofs Freeable.
+  valid_access m2 chunk b ofs Freeable c.
 Proof.
   intros. constructor; auto with mem.
   red; intros. apply perm_alloc_2. omega.
+  split.
+  apply owned_new_block.
+  auto.
 Qed.
 
 Local Hint Resolve valid_access_alloc_other valid_access_alloc_same: mem.
 
 Theorem valid_access_alloc_inv:
-  forall chunk b' ofs p,
-  valid_access m2 chunk b' ofs p ->
+  forall chunk b' ofs p c',
+  valid_access m2 chunk b' ofs p c' ->
   if eq_block b' b
   then lo <= ofs /\ ofs + size_chunk chunk <= hi /\ (align_chunk chunk | ofs)
-  else valid_access m1 chunk b' ofs p.
+  else valid_access m1 chunk b' ofs p c'.
 Proof.
-  intros. inv H.
+  intros. inv H. destruct H1 as [H1 Hx].
   generalize (size_chunk_pos chunk); intro.
   destruct (eq_block b' b). subst b'.
   assert (perm m2 b ofs Cur p). apply H0. omega.
@@ -1885,12 +2137,15 @@ Proof.
   intuition omega.
   split; auto. red; intros.
   exploit perm_alloc_inv. apply H0. eauto. rewrite dec_eq_false; auto.
+  split.
+  apply alloc_own_block_other_inj_2; assumption.
+  assumption.
 Qed.
 
 Theorem load_alloc_unchanged:
-  forall chunk b' ofs,
+  forall chunk b' ofs c',
   valid_block m1 b' ->
-  load chunk m2 b' ofs = load chunk m1 b' ofs.
+  load chunk m2 b' ofs c' = load chunk m1 b' ofs c'.
 Proof.
   intros. unfold load.
   destruct (valid_access_dec m2 chunk b' ofs Readable).
@@ -1904,16 +2159,16 @@ Proof.
 Qed.
 
 Theorem load_alloc_other:
-  forall chunk b' ofs v,
-  load chunk m1 b' ofs = Some v ->
-  load chunk m2 b' ofs = Some v.
+  forall chunk b' ofs c' v,
+  load chunk m1 b' ofs c' = Some v ->
+  load chunk m2 b' ofs c' = Some v.
 Proof.
   intros. rewrite <- H. apply load_alloc_unchanged. eauto with mem.
 Qed.
 
 Theorem load_alloc_same:
-  forall chunk ofs v,
-  load chunk m2 b ofs = Some v ->
+  forall chunk ofs c' v,
+  load chunk m2 b ofs c' = Some v ->
   v = Vundef.
 Proof.
   intros. exploit load_result; eauto. intro. rewrite H0.
@@ -1922,39 +2177,54 @@ Proof.
   rewrite ZMap.gi. apply decode_val_undef.
 Qed.
 
+(* RB: NOTE: In keeping with the style of the lemma, we add the missing
+   assumption to it, however it is unclear whether this is the best choice.
+   Clearly, c' can only be c, and block ownership can be established from
+   known facts. *)
 Theorem load_alloc_same':
-  forall chunk ofs,
-  lo <= ofs -> ofs + size_chunk chunk <= hi -> (align_chunk chunk | ofs) ->
-  load chunk m2 b ofs = Some Vundef.
+  forall chunk ofs c',
+  lo <= ofs -> ofs + size_chunk chunk <= hi -> own_block m2 b c' -> (align_chunk chunk | ofs) ->
+  load chunk m2 b ofs c' = Some Vundef.
 Proof.
-  intros. assert (exists v, load chunk m2 b ofs = Some v).
+  intros. assert (exists v, load chunk m2 b ofs c' = Some v).
     apply valid_access_load. constructor; auto.
     red; intros. eapply perm_implies. apply perm_alloc_2. omega. auto with mem.
-  destruct H2 as [v LOAD]. rewrite LOAD. decEq.
+  destruct H3 as [v LOAD]. rewrite LOAD. decEq.
   eapply load_alloc_same; eauto.
 Qed.
 
 Theorem loadbytes_alloc_unchanged:
-  forall b' ofs n,
+  forall b' ofs n c',
   valid_block m1 b' ->
-  loadbytes m2 b' ofs n = loadbytes m1 b' ofs n.
+  loadbytes m2 b' ofs n c' = loadbytes m1 b' ofs n c'.
 Proof.
   intros. unfold loadbytes.
   destruct (range_perm_dec m1 b' ofs (ofs + n) Cur Readable).
-  rewrite pred_dec_true.
+- destruct (own_block_dec m1 b' c').
++ setoid_rewrite pred_dec_true. simpl.
   injection ALLOC; intros A B. rewrite <- B; simpl.
   rewrite PMap.gso. auto. rewrite A. eauto with mem.
   red; intros. eapply perm_alloc_1; eauto.
-  rewrite pred_dec_false; auto.
+  apply alloc_own_block_other_inj_1; assumption.
++ setoid_rewrite pred_dec_false at 2.
+* rewrite andb_comm. reflexivity.
+* intro Hcontra. apply n0.
+  apply alloc_own_block_other_inj_2; auto.
+  apply valid_block_alloc_inv'; assumption.
+- setoid_rewrite pred_dec_false at 1; auto.
   red; intros; elim n0. red; intros. eapply perm_alloc_4; eauto. eauto with mem.
 Qed.
 
+(* RB: NOTE: Could also use c here. *)
 Theorem loadbytes_alloc_same:
-  forall n ofs bytes byte,
-  loadbytes m2 b ofs n = Some bytes ->
+  forall n ofs c' bytes byte,
+  loadbytes m2 b ofs n c' = Some bytes ->
   In byte bytes -> byte = Undef.
 Proof.
-  unfold loadbytes; intros. destruct (range_perm_dec m2 b ofs (ofs + n) Cur Readable); inv H.
+  unfold loadbytes; intros.
+  destruct (range_perm_dec m2 b ofs (ofs + n) Cur Readable);
+  destruct (own_block_dec m2 b c');
+  inv H.
   revert H0.
   injection ALLOC; intros A B. rewrite <- A; rewrite <- B; simpl. rewrite PMap.gss.
   generalize (Z.to_nat n) ofs. induction n0; simpl; intros.
